Makefile
@@ -1,4 +1,4 @@
-FSTAR_HOME=/home/yannick/Code/fstar
+FSTAR_HOME=/home/yannick/Code/fstar-lang
 FSTAR_BIN=fstar
 FSTAR=$(FSTAR_HOME)/bin/$(FSTAR_BIN) --n_cores 1 --max_fuel 1 --max_ifuel 1 --fstar_home $(FSTAR_HOME) --print_implicits
 
